Refactoring RST, a general notion of constructive resource inclusion, swap examples both in left/right and inclusion style

ulib/LowStar.RST.fst
@@ -27,68 +27,64 @@ let imem inv = m:HS.mem{inv m}
 let eloc = Ghost.erased B.loc
 let as_loc (x:eloc) : GTot B.loc = Ghost.reveal x
 
-let view_t a b = a -> GTot b
 
-let view_reads_fp #b fp #inv (view:view_t (imem inv) b) =
-  forall (h0 h1:imem inv) loc. {:pattern  (B.modifies loc h0 h1); (view h1)}
+let sel_reads_fp #b fp #inv (sel:(imem inv) -> GTot b) =
+  forall (h0 h1:imem inv) loc. {:pattern  (B.modifies loc h0 h1); (sel h1)}
     B.loc_disjoint (as_loc fp) loc /\
     B.modifies loc h0 h1 ==>
-    view h0 == view h1
+    sel h0 == sel h1
 
-let r_view_t fp inv a =
-  sel:view_t (imem inv) a {
-    view_reads_fp fp sel
-  }
-
-noeq
-type r_view fp inv : Type u#1 = {
-    t: Type0;
-    sel: r_view_t fp inv t
-  }
-
-noeq
-type resource_t : Type u#1 = {
-    fp: eloc;
-    inv: HS.mem -> Type0;
-    view: r_view fp inv         // might become a list of (r_view inv fp)'s one day
-  }
-
-let invariant_reads_fp fp inv =
+let inv_reads_fp fp inv =
   forall h0 h1 loc.{:pattern (B.modifies loc h0 h1); (inv h1)}
     inv h0 /\
     B.loc_disjoint (as_loc fp) loc /\
     B.modifies loc h0 h1 ==>
     inv h1
 
-let resource =
-  res:resource_t {
-    invariant_reads_fp res.fp res.inv
+unfold
+let view_t a b = a -> GTot b
+
+noeq 
+type view_aux a = {
+    fp: eloc;
+    inv: HS.mem -> Type0;
+    sel: view_t (imem inv) a
   }
 
-abstract
-let inv (res:resource) (h:HS.mem) =
-  res.inv h
+let view a = 
+  view:view_aux a{
+    sel_reads_fp view.fp view.sel /\
+    inv_reads_fp view.fp view.inv
+  }
+
+noeq 
+type resource : Type u#1 = {
+    t: Type u#0;
+    view: view t
+  }
+
+let as_resource (#a:Type) (view:view a) : resource = {
+    t = a;
+    view = view
+  }
+
+let view_of (res:resource) = 
+  res.view
 
 abstract
 let fp (res:resource) = 
-  res.fp
-
-type view a = {
-  fp:loc;
-  inv:mem -> prop;
-  sel:imem -> a
-}
-
-resource = (a:Type * view a)
-
-sel (v:view a) (h:imem (singleton v)) : a
+  res.view.fp
 
 abstract
-let sel (res:resource) (h:imem (inv res)) =
-  res.view.sel h
+let inv (res:resource) (h:HS.mem) =
+  res.view.inv h
 
 abstract
-let modifies (res:resource) (h0 h1: HS.mem) =
+let sel (#a:Type) (view:view a) (h:imem (inv (as_resource view))) =
+  view.sel h
+
+abstract
+let modifies (res:resource) (h0 h1:HS.mem) =
     B.modifies (as_loc (fp res)) h0 h1 /\
     HST.equal_domains h0 h1
 
@@ -100,12 +96,13 @@ let modifies_trans (res:resource) (h0 h1 h2:HS.mem)
              modifies res h0 h2)
            [SMTPat (modifies res h0 h2);
             SMTPat (modifies res h0 h1)]
-  = ()            
+  = ()
 
 let reveal ()
-  : Lemma ((forall res h .{:pattern inv res h} inv res h <==> res.inv h) /\ 
-           (forall res .{:pattern fp res} fp res == res.fp) /\ 
-           (forall res h .{:pattern sel res h} sel res h == res.view.sel h) /\
+  : Lemma ((forall res.{:pattern view_of res} view_of res == res.view) /\
+           (forall res h .{:pattern inv res h} inv res h <==> res.view.inv h) /\ 
+           (forall res .{:pattern fp res} fp res == res.view.fp) /\ 
+           (forall a (view:view a) h .{:pattern sel view h} sel view h == view.sel h) /\
            (forall res h0 h1.{:pattern modifies res h0 h1}
              modifies res h0 h1 <==>
              B.modifies (as_loc (fp res)) h0 h1 /\
@@ -119,79 +116,76 @@ let r_disjoint (res1 res2:resource) =
   B.loc_disjoint (as_loc (fp res1)) (as_loc (fp res2))
 
 abstract
-let ( <*> ) (res1 res2:resource) : res:resource{res.view.t == res1.view.t & res2.view.t} = 
+let ( <*> ) (res1 res2:resource) : res:resource = 
   let fp = Ghost.hide (B.loc_union (as_loc (fp res1)) (as_loc (fp res2))) in 
   let inv h = inv res1 h /\ inv res2 h /\ r_disjoint res1 res2 in
-  let view = (
-    let t = res1.view.t & res2.view.t in 
-    let sel h = (sel res1 h,sel res2 h) in 
-    {
-      t = t;
+  let sel h = (sel res1.view h,sel res2.view h) in
+  let t = res1.t & res2.t in 
+  let view = {
+      fp = fp;
+      inv = inv;
       sel = sel
-    }) in
+    } in 
   {
-    fp = fp;
-    inv = inv;
+    t = t;
     view = view
   }
 
 let reveal_star_inv (res1 res2:resource) (h:HS.mem)
-  : Lemma ((inv (res1 <*> res2) h) <==> (inv res1 h /\ inv res2 h /\ r_disjoint res1 res2))
-          [SMTPat (inv (res1 <*> res2) h)] = 
+  : Lemma ((inv (res1 <*> res2) h) 
+           <==> 
+           (inv res1 h /\ inv res2 h /\ r_disjoint res1 res2))
+          [SMTPat (inv (res1 <*> res2) h)] =                    // [DA: we might consider removing this SMTPat 
+                                                                //      at the cost of having to have expicitly 
+                                                                //      call reveals in specs involving <*>]
   ()
 
-let reveal_star_fp (res1 res2:resource) 
-  : Lemma (as_loc (fp (res1 <*> res2)) == B.loc_union (as_loc (fp res1)) (as_loc (fp res2))) = 
+let reveal_star (res1 res2:resource) 
+  : Lemma (as_loc (fp (res1 <*> res2)) == B.loc_union (as_loc (fp res1)) (as_loc (fp res2)) /\
+           (res1 <*> res2).t == res1.t & res2.t) = 
   ()
 
-let reveal_star_view_t (res1 res2:resource)
-  : Lemma ((res1 <*> res2).view.t == res1.view.t & res2.view.t) = 
-  ()
-
-(* (Constructive) view and resource inclusion *)
+(* Constructive resource inclusion *)
 
 noeq
 type r_includes_t (res1 res2:resource) = {
-    view_inc: res1.view.t -> res2.view.t;
-    fp_delta: eloc
+    inc: view_t res1.t res2.t;   // viewing larger resource as a smaller one
+    delta: resource              // delta separating the two resources
   }
 
-let r_includes res1 res2 =
+let r_includes res1 res2 = 
   inc:r_includes_t res1 res2 {
-    // Difference in resource footprints is exactly inc.fp_delta
-    (B.loc_disjoint (as_loc inc.fp_delta) (as_loc (fp res2))) /\ 
-    (as_loc (fp res1) == B.loc_union (as_loc inc.fp_delta) (as_loc (fp res2))) /\
-    // Larger resource's invariant implies the smaller resource's one (e.g., liveness)
-    (forall h .{:pattern (inv res1 h); (inv res2 h)} inv res1 h ==> inv res2 h) /\
     // Views are mapped to views
-    (forall h .{:pattern (inc.view_inc (sel res1 h))} 
-               inc.view_inc (sel res1 h) == sel res2 h) /\
-    // Larger resource's invariant can be framed across modifications by the smaller resource
-    (forall h0 h1 .{:pattern (inv res1 h1); (B.modifies (as_loc (fp res2)) h0 h1)} 
-                   inv res1 h0 /\ B.modifies (as_loc (fp res2)) h0 h1 /\ inv res2 h1 ==> inv res1 h1)
-                   // [DA: can we get rid of this modifies somehow?]
+    (forall h .{:pattern (inc.inc (sel (view_of res1) h))} 
+               inc.inc (sel (view_of res1) h) == sel (view_of res2) h) /\
+    // Delta is disjoint from the smaller resource
+    r_disjoint inc.delta res2 /\
+    // Footprint of the larger resource is union of delta and the smaller resource
+    as_loc (fp res1) == B.loc_union (as_loc (fp inc.delta)) (as_loc (fp res2)) /\
+    // Larger resource's invariant implies the smaller resource's invariant (e.g., liveness)
+    (forall h .{:pattern (inv res1 h); (inv res2 h)} inv res1 h ==> inv res2 h) /\
+    // Larger invariant is equivalent to delta and the smaller invariant
+    (forall h . inv res1 h <==> inv res2 h /\ inv inc.delta h)
   }
 
 (* Left and right inclusions for separating conjunction *)
 
-let star_includes_left (res1:resource) 
-                       (res2:resource{B.loc_disjoint (as_loc (fp res1)) (as_loc (fp res2))})
-                     : r_includes (res1 <*> res2) res1 = 
-  let view_inc (xy:(res1 <*> res2).view.t) = fst xy in 
-  let fp_delta = fp res2 in
+let star_includes_left (#fp:resource) 
+                       (frame:resource{r_disjoint fp frame})
+                     : r_includes (fp <*> frame) fp = 
+  let inc (xy:(fp <*> frame).t) = fst xy in 
   {
-    view_inc = view_inc;
-    fp_delta = fp_delta
+    inc = inc;
+    delta = frame
   }
 
-let star_includes_right (res1:resource) 
-                        (res2:resource{B.loc_disjoint (as_loc (fp res1)) (as_loc (fp res2))})
-                      : r_includes (res1 <*> res2) res2 = 
-  let view_inc (xy:(res1 <*> res2).view.t) = snd xy in 
-  let fp_delta = fp res1 in
+let star_includes_right (#fp:resource) 
+                        (frame:resource{r_disjoint frame fp})
+                      : r_includes (frame <*> fp) fp = 
+  let inc (xy:(frame <*> fp).t) = snd xy in 
   {
-    view_inc = view_inc;
-    fp_delta = fp_delta
+    inc = inc;
+    delta = frame
   }
 
 (* State effect indexed by a resource *)
@@ -214,33 +208,25 @@ effect RST (a:Type)
                  post h0 x h1 ==>                       //Ensure the post-condition
                  k x h1))                               //prove the continuation under this hypothesis
 
-(* Simple packaging of resources with readers-writers for them *)
-noeq
-type resource_w_rw = {
-    res: resource;
-    reader: unit -> RST (res.view.t) res (fun _ -> True) (fun h0 x h1 -> sel res h0 == x /\ x == sel res h1);
-    writer: x:res.view.t -> RST unit res (fun _ -> True) (fun _ _ h1 -> sel res h1 == x)
-  }
-
-(* Framing for RST computations *)
+(* Left and right framing operations for RST computations *)
 
 unfold
-let frame_left_pre (#res1:resource)
-              (#res2:resource)
-              (pre:r_pre res1)
-              (h:imem (inv (res1 <*> res2))) = 
+let frame_left_pre (#fp:resource)
+              (#frame:resource)
+              (pre:r_pre fp)
+              (h:imem (inv (fp <*> frame))) = 
   pre h
 
 unfold
-let frame_left_post (#res1:resource)
-               (#res2:resource)
+let frame_left_post (#fp:resource)
+               (#frame:resource)
                (#a:Type)
-               (post:r_post res1 a)
-               (h0:imem (inv (res1 <*> res2)))
+               (post:r_post fp a)
+               (h0:imem (inv (fp <*> frame)))
                (x:a)
-               (h1:imem (inv (res1 <*> res2))) =
+               (h1:imem (inv (fp <*> frame))) =
   post h0 x h1 /\
-  sel res2 h0 == sel res2 h1
+  sel (view_of frame) h0 == sel (view_of frame) h1
 
 let frame_left 
           (#frame:resource)
@@ -255,22 +241,22 @@ let frame_left
   f ()
 
 unfold
-let frame_right_pre (#res1:resource)
-               (#res2:resource)
-               (pre:r_pre res2)
-               (h:imem (inv (res1 <*> res2))) = 
+let frame_right_pre (#frame:resource)
+               (#fp:resource)
+               (pre:r_pre fp)
+               (h:imem (inv (frame <*> fp))) = 
   pre h
 
 unfold
-let frame_right_post (#res1:resource)
-                (#res2:resource)
+let frame_right_post (#frame:resource)
+                (#fp:resource)
                 (#a:Type)
-                (post:r_post res2 a)
-                (h0:imem (inv (res1 <*> res2)))
+                (post:r_post fp a)
+                (h0:imem (inv (frame <*> fp)))
                 (x:a)
-                (h1:imem (inv (res1 <*> res2))) =
+                (h1:imem (inv (frame <*> fp))) =
   post h0 x h1 /\
-  sel res1 h0 == sel res1 h1
+  sel (view_of frame) h0 == sel (view_of frame) h1
 
 let frame_right 
            (#frame:resource)
@@ -284,33 +270,35 @@ let frame_right
                  (frame_right_post post) =
   f ()
 
-(* Resource inclusion for RST computations *)
+(* Generic frame operation for RST computations (through resource inclusion) *)
+
 unfold
-let include_pre (#res1:resource)
-                (#res2:resource)
-                (inc:r_includes res1 res2)
-                (pre:r_pre res2)
-                (h:imem (inv res1)) =
+let frame_pre (#outer:resource)
+                (#inner:resource)
+                (inc:r_includes outer inner)
+                (pre:r_pre inner)
+                (h:imem (inv outer)) =
   pre h
 
 unfold
-let include_post (#res1:resource)
-                 (#res2:resource)
-                 (inc:r_includes res1 res2)
+let frame_post (#outer:resource)
+                 (#inner:resource)
+                 (inc:r_includes outer inner)
                  (#a:Type)
-                 (post:r_post res2 a)
-                 (h0:imem (inv res1))
+                 (post:r_post inner a)
+                 (h0:imem (inv outer))
                  (x:a)
-                 (h1:imem (inv res1)) = 
-  (post h0 x h1) /\
-  (B.modifies (as_loc (fp res2)) h0 h1) // [DA: can we get rid of this modifies somehow?]
-
-let r_include (#a:Type)
-              (#res1:resource)
-              (#res2:resource)
-              (inc:r_includes res1 res2)
-              (#pre:r_pre res2)
-              (#post:r_post res2 a)
-              ($f:unit -> RST a res2 pre post)
-            : RST a res1 (include_pre inc pre) (include_post inc post) =
+                 (h1:imem (inv outer)) = 
+  post h0 x h1 /\
+  sel (view_of inc.delta) h0 == sel (view_of inc.delta) h1
+  
+let frame (#a:Type)
+              (#outer:resource)
+              (#inner:resource)
+              (inc:r_includes outer inner)  // eventually we will want to infer this argument through metaprogramming
+              (#pre:r_pre inner)
+              (#post:r_post inner a)
+              ($f:unit -> RST a inner pre post)
+            : RST a outer (frame_pre inc pre) (frame_post inc post) =
   f ()
+
